seiostar/LambdaIO.DestructLemmas.fst
@@ -187,7 +187,7 @@ let can_step_eif_when_safe (e1 e2 e3:closed_exp) (h:history) : Lemma
     end
   end
 
-#push-options "--split_queries always"
+#push-options "--z3rlimit 10"
 let rec destruct_steps_eif
   (e1:closed_exp)
   (e2:closed_exp)
@@ -243,6 +243,7 @@ let rec destruct_steps_eif
         (e1, (| [], lt |))
         end
       end
+
 #pop-options
 
   (**
@@ -268,7 +269,7 @@ let lem_irred_epair_implies_irred_e2 (e1':closed_exp{is_value e1'}) (e2:closed_e
     end
   end
 
-#push-options "--split_queries always"
+#push-options "--z3rlimit 10"
 let rec destruct_steps_epair_e1
   (e1:closed_exp)
   (e2:closed_exp)
@@ -319,7 +320,7 @@ let rec destruct_steps_epair_e1
     end
 #pop-options
 
-#push-options "--split_queries always"
+#push-options "--z3rlimit 10"
 let rec destruct_steps_epair_e2
   (e1':closed_exp{is_value e1'})
   (e2:closed_exp)
@@ -408,7 +409,7 @@ let lem_irred_estringeq_implies_irred_e2 (e1':closed_exp{EString? e1'}) (e2:clos
     end
   end
 
-#push-options "--split_queries always"
+#push-options "--z3rlimit 10"
 let rec destruct_steps_estringeq_e1
   (e1:closed_exp)
   (e2:closed_exp)
